impl/riscv/mont_mul_lemmas.i.dfy
@@ -1,0 +1,52 @@
+include "mont_mul_add_lemmas.i.dfy"
+
+module mont_mul_lemmas {
+    import opened bv_ops
+    import opened rsa_ops
+    import opened rv_machine
+
+    import opened BASE_32_Seq
+    import opened Mul
+    import Power2
+    import Power
+    import opened DivMod
+    
+    import opened mont_mul_add_lemmas
+
+    datatype mm_vars = mm_vars(
+        mm_frame_ptr: uint32, // writable
+        mma_frame_ptr: uint32, // writable
+        iter_a: iter_t,
+        iter_b: iter_t,
+        iter_c: iter_t, // writable
+        iter_n: iter_t
+    )
+
+    function to_mma_vars(vars: mm_vars, a_i: uint32): mma_vars
+    {
+        mma_vars(vars.mma_frame_ptr,
+            vars.iter_a, a_i, vars.iter_a.index,
+            vars.iter_b, vars.iter_c, vars.iter_n)
+    }
+
+    predicate mm_vars_inv(
+        vars: mm_vars,
+        mem: mem_t,
+        a_ptr: int, a_idx: int,
+        n_ptr: int, n_idx: int,
+        c_ptr: int, c_idx: int,
+        b_ptr: int, b_idx: int,
+        rsa: rsa_params)
+    {
+        && mvar_iter_inv(mem, vars.iter_a, a_ptr, a_idx, NA)
+        && var a_i := if 0 <= a_idx < NUM_WORDS then vars.iter_a.buff[a_idx] else 0;
+        && var mma := to_mma_vars(vars, a_i);
+        && mma_vars_inv(mma, mem, n_ptr, n_idx, c_ptr, c_idx, b_ptr, b_idx, rsa)
+        && valid_frame_ptr(mem, vars.mm_frame_ptr, 12)
+        && vars.mm_frame_ptr != vars.mma_frame_ptr
+        && vars.mm_frame_ptr != vars.iter_a.base_addr
+        && vars.mm_frame_ptr != vars.iter_b.base_addr
+        && vars.mm_frame_ptr != vars.iter_c.base_addr
+        && vars.mm_frame_ptr != vars.iter_n.base_addr
+    }
+}
